FormalHdl/Adder.lean
@@ -1,0 +1,278 @@
+-- Adam Friesz, Winter 2026
+import FormalHdl.Defs
+namespace hdl.examples.adder
+open hdl
+set_option linter.style.longLine false
+set_option linter.style.whitespace false
+
+
+-- COMPONENT: adder_rca_1
+def adder_rca_1_gates : List Gate := [
+  Gate.mk .igate false,
+  Gate.mk .igate false,
+  Gate.mk .igate false,
+  Gate.mk .xor_ false,
+  Gate.mk .and_ false,
+  Gate.mk .xor_ false,
+  Gate.mk .and_ false,
+  Gate.mk .or_ false
+]
+def adder_rca_1_conns : List (List Nat) := [
+  [],
+  [],
+  [],
+  [1, 2],
+  [1, 2],
+  [3, 0],
+  [3, 0],
+  [4, 6]
+]
+def adder_rca_1 : Circuit := { gates := adder_rca_1_gates, wiring := mkWiring adder_rca_1_gates adder_rca_1_conns (by decide), is_dag := by decide }
+def a_bus_adder_rca_1 : List (Fin 8) := [⟨1, by decide⟩]
+def b_bus_adder_rca_1 : List (Fin 8) := [⟨2, by decide⟩]
+def sum_bus_adder_rca_1 : List (Fin 8) := [⟨5, by decide⟩]
+def cin_adder_rca_1 : Fin 8 := ⟨0, by decide⟩
+def cout_adder_rca_1 : Fin 8 := ⟨7, by decide⟩
+
+-- AST BOUNDARY LEMMAS & PROOF: adder_rca_1
+@[simp] lemma ast_adder_rca_1_cin (s : State adder_rca_1) (i : Fin 8) (hi : i.val = 0 := by decide) : evalExpr s (unrollDAG adder_rca_1 8 i) = s ⟨0, by decide⟩ := by cases i; subst hi; rfl
+@[simp] lemma ast_adder_rca_1_a_0 (s : State adder_rca_1) (i : Fin 8) (hi : i.val = 1 := by decide) : evalExpr s (unrollDAG adder_rca_1 8 i) = s ⟨1, by decide⟩ := by cases i; subst hi; rfl
+@[simp] lemma ast_adder_rca_1_b_0 (s : State adder_rca_1) (i : Fin 8) (hi : i.val = 2 := by decide) : evalExpr s (unrollDAG adder_rca_1 8 i) = s ⟨2, by decide⟩ := by cases i; subst hi; rfl
+@[simp] lemma ast_adder_rca_1_sum_0 (s : State adder_rca_1) (i : Fin 8) (hi : i.val = 5 := by decide) : evalExpr s (unrollDAG adder_rca_1 8 i) = ((s ⟨1, by decide⟩ ^^ s ⟨2, by decide⟩) ^^ s ⟨0, by decide⟩) := by cases i; subst hi; rfl
+@[simp] lemma ast_adder_rca_1_cout (s : State adder_rca_1) (i : Fin 8) (hi : i.val = 7 := by decide) : evalExpr s (unrollDAG adder_rca_1 8 i) = ((s ⟨1, by decide⟩ && s ⟨2, by decide⟩) || ((s ⟨1, by decide⟩ ^^ s ⟨2, by decide⟩) && s ⟨0, by decide⟩)) := by cases i; subst hi; rfl
+
+instance instIsAdder_adder_rca_1 : IsAdder adder_rca_1 1 a_bus_adder_rca_1 b_bus_adder_rca_1 sum_bus_adder_rca_1 cin_adder_rca_1 cout_adder_rca_1 where
+  widths_match := by decide
+  inputs_are_valid := by intro i h; fin_cases h <;> rfl
+  adder_correct := by
+    intro s
+    have equiv (i : Fin 8) : evalCombinatorial adder_rca_1 adder_rca_1.gates.length s i = evalExpr s (unrollDAG adder_rca_1 8 i) := by fin_cases i <;> rfl
+    simp only [a_bus_adder_rca_1, b_bus_adder_rca_1, sum_bus_adder_rca_1, cout_adder_rca_1, cin_adder_rca_1, bitsToNat]
+    simp only [equiv]
+    simp only [ast_adder_rca_1_cin, ast_adder_rca_1_a_0, ast_adder_rca_1_b_0, ast_adder_rca_1_sum_0, ast_adder_rca_1_cout]
+    generalize h_cin : s ⟨0, by decide⟩ = cin
+    generalize h_a_0 : s ⟨1, by decide⟩ = a_0
+    generalize h_b_0 : s ⟨2, by decide⟩ = b_0
+    cases cin <;> cases a_0 <;> cases b_0 <;> decide
+
+instance instVerifiedAdder1_adder_rca_1 : VerifiedAdder1 adder_rca_1 a_bus_adder_rca_1 b_bus_adder_rca_1 sum_bus_adder_rca_1 cin_adder_rca_1 cout_adder_rca_1 where
+  proof := instIsAdder_adder_rca_1
+
+-- COMPONENT: adder_hierarchical_2
+def adder_hierarchical_2_gates : List Gate := [
+  Gate.mk .igate false,
+  Gate.mk .igate false,
+  Gate.mk .igate false,
+  Gate.mk .igate false,
+  Gate.mk .igate false,
+  Gate.mk (.adder_1 ⟨0, by decide⟩) false,
+  Gate.mk (.adder_1 ⟨1, by decide⟩) false,
+  Gate.mk (.adder_1 ⟨0, by decide⟩) false,
+  Gate.mk (.adder_1 ⟨1, by decide⟩) false
+]
+def adder_hierarchical_2_conns : List (List Nat) := [
+  [],
+  [],
+  [],
+  [],
+  [],
+  [0, 1, 2],
+  [0, 1, 2],
+  [6, 3, 4],
+  [6, 3, 4]
+]
+def adder_hierarchical_2 : Circuit := { gates := adder_hierarchical_2_gates, wiring := mkWiring adder_hierarchical_2_gates adder_hierarchical_2_conns (by decide), is_dag := by decide }
+def a_bus_adder_hierarchical_2 : List (Fin 9) := [⟨1, by decide⟩, ⟨3, by decide⟩]
+def b_bus_adder_hierarchical_2 : List (Fin 9) := [⟨2, by decide⟩, ⟨4, by decide⟩]
+def sum_bus_adder_hierarchical_2 : List (Fin 9) := [⟨5, by decide⟩, ⟨7, by decide⟩]
+def cin_adder_hierarchical_2 : Fin 9 := ⟨0, by decide⟩
+def cout_adder_hierarchical_2 : Fin 9 := ⟨8, by decide⟩
+
+-- AST BOUNDARY LEMMAS & PROOF: adder_hierarchical_2
+@[simp] lemma ast_adder_hierarchical_2_cin (s : State adder_hierarchical_2) (i : Fin 9) (hi : i.val = 0 := by decide) : evalExpr s (unrollDAG adder_hierarchical_2 9 i) = s ⟨0, by decide⟩ := by cases i; subst hi; rfl
+@[simp] lemma ast_adder_hierarchical_2_a_0 (s : State adder_hierarchical_2) (i : Fin 9) (hi : i.val = 1 := by decide) : evalExpr s (unrollDAG adder_hierarchical_2 9 i) = s ⟨1, by decide⟩ := by cases i; subst hi; rfl
+@[simp] lemma ast_adder_hierarchical_2_b_0 (s : State adder_hierarchical_2) (i : Fin 9) (hi : i.val = 2 := by decide) : evalExpr s (unrollDAG adder_hierarchical_2 9 i) = s ⟨2, by decide⟩ := by cases i; subst hi; rfl
+@[simp] lemma ast_adder_hierarchical_2_a_1 (s : State adder_hierarchical_2) (i : Fin 9) (hi : i.val = 3 := by decide) : evalExpr s (unrollDAG adder_hierarchical_2 9 i) = s ⟨3, by decide⟩ := by cases i; subst hi; rfl
+@[simp] lemma ast_adder_hierarchical_2_b_1 (s : State adder_hierarchical_2) (i : Fin 9) (hi : i.val = 4 := by decide) : evalExpr s (unrollDAG adder_hierarchical_2 9 i) = s ⟨4, by decide⟩ := by cases i; subst hi; rfl
+@[simp] lemma ast_adder_hierarchical_2_sum_0 (s : State adder_hierarchical_2) (i : Fin 9) (hi : i.val = 5 := by decide) : evalExpr s (unrollDAG adder_hierarchical_2 9 i) = (compute_adder_1 (s ⟨0, by decide⟩) (s ⟨1, by decide⟩) (s ⟨2, by decide⟩)).testBit 0 := by cases i; subst hi; rfl
+@[simp] lemma ast_adder_hierarchical_2_sum_1 (s : State adder_hierarchical_2) (i : Fin 9) (hi : i.val = 7 := by decide) : evalExpr s (unrollDAG adder_hierarchical_2 9 i) = (compute_adder_1 ((compute_adder_1 (s ⟨0, by decide⟩) (s ⟨1, by decide⟩) (s ⟨2, by decide⟩)).testBit 1) (s ⟨3, by decide⟩) (s ⟨4, by decide⟩)).testBit 0 := by cases i; subst hi; rfl
+@[simp] lemma ast_adder_hierarchical_2_cout (s : State adder_hierarchical_2) (i : Fin 9) (hi : i.val = 8 := by decide) : evalExpr s (unrollDAG adder_hierarchical_2 9 i) = (compute_adder_1 ((compute_adder_1 (s ⟨0, by decide⟩) (s ⟨1, by decide⟩) (s ⟨2, by decide⟩)).testBit 1) (s ⟨3, by decide⟩) (s ⟨4, by decide⟩)).testBit 1 := by cases i; subst hi; rfl
+
+instance instIsAdder_adder_hierarchical_2 : IsAdder adder_hierarchical_2 2 a_bus_adder_hierarchical_2 b_bus_adder_hierarchical_2 sum_bus_adder_hierarchical_2 cin_adder_hierarchical_2 cout_adder_hierarchical_2 where
+  widths_match := by decide
+  inputs_are_valid := by intro i h; fin_cases h <;> rfl
+  adder_correct := by
+    intro s
+    have equiv (i : Fin 9) : evalCombinatorial adder_hierarchical_2 adder_hierarchical_2.gates.length s i = evalExpr s (unrollDAG adder_hierarchical_2 9 i) := by fin_cases i <;> rfl
+    simp only [a_bus_adder_hierarchical_2, b_bus_adder_hierarchical_2, sum_bus_adder_hierarchical_2, cout_adder_hierarchical_2, cin_adder_hierarchical_2, bitsToNat]
+    simp only [equiv]
+    simp only [ast_adder_hierarchical_2_cin, ast_adder_hierarchical_2_a_0, ast_adder_hierarchical_2_b_0, ast_adder_hierarchical_2_a_1, ast_adder_hierarchical_2_b_1, ast_adder_hierarchical_2_sum_0, ast_adder_hierarchical_2_sum_1, ast_adder_hierarchical_2_cout]
+    generalize h_cin : s ⟨0, by decide⟩ = cin
+    generalize h_a_0 : s ⟨1, by decide⟩ = a_0
+    generalize h_b_0 : s ⟨2, by decide⟩ = b_0
+    generalize h_a_1 : s ⟨3, by decide⟩ = a_1
+    generalize h_b_1 : s ⟨4, by decide⟩ = b_1
+    cases cin <;> cases a_0 <;> cases b_0 <;> cases a_1 <;> cases b_1 <;> decide
+
+instance instVerifiedAdder2_adder_hierarchical_2 : VerifiedAdder2 adder_hierarchical_2 a_bus_adder_hierarchical_2 b_bus_adder_hierarchical_2 sum_bus_adder_hierarchical_2 cin_adder_hierarchical_2 cout_adder_hierarchical_2 where
+  proof := instIsAdder_adder_hierarchical_2
+
+-- COMPONENT: adder_hierarchical_4
+def adder_hierarchical_4_gates : List Gate := [
+  Gate.mk .igate false,
+  Gate.mk .igate false,
+  Gate.mk .igate false,
+  Gate.mk .igate false,
+  Gate.mk .igate false,
+  Gate.mk .igate false,
+  Gate.mk .igate false,
+  Gate.mk .igate false,
+  Gate.mk .igate false,
+  Gate.mk (.adder_2 ⟨0, by decide⟩) false,
+  Gate.mk (.adder_2 ⟨1, by decide⟩) false,
+  Gate.mk (.adder_2 ⟨2, by decide⟩) false,
+  Gate.mk (.adder_2 ⟨0, by decide⟩) false,
+  Gate.mk (.adder_2 ⟨1, by decide⟩) false,
+  Gate.mk (.adder_2 ⟨2, by decide⟩) false
+]
+def adder_hierarchical_4_conns : List (List Nat) := [
+  [],
+  [],
+  [],
+  [],
+  [],
+  [],
+  [],
+  [],
+  [],
+  [0, 1, 3, 2, 4],
+  [0, 1, 3, 2, 4],
+  [0, 1, 3, 2, 4],
+  [11, 5, 7, 6, 8],
+  [11, 5, 7, 6, 8],
+  [11, 5, 7, 6, 8]
+]
+def adder_hierarchical_4 : Circuit := { gates := adder_hierarchical_4_gates, wiring := mkWiring adder_hierarchical_4_gates adder_hierarchical_4_conns (by decide), is_dag := by decide }
+def a_bus_adder_hierarchical_4 : List (Fin 15) := [⟨1, by decide⟩, ⟨3, by decide⟩, ⟨5, by decide⟩, ⟨7, by decide⟩]
+def b_bus_adder_hierarchical_4 : List (Fin 15) := [⟨2, by decide⟩, ⟨4, by decide⟩, ⟨6, by decide⟩, ⟨8, by decide⟩]
+def sum_bus_adder_hierarchical_4 : List (Fin 15) := [⟨9, by decide⟩, ⟨10, by decide⟩, ⟨12, by decide⟩, ⟨13, by decide⟩]
+def cin_adder_hierarchical_4 : Fin 15 := ⟨0, by decide⟩
+def cout_adder_hierarchical_4 : Fin 15 := ⟨14, by decide⟩
+
+-- AST BOUNDARY LEMMAS & PROOF: adder_hierarchical_4
+@[simp] lemma ast_adder_hierarchical_4_cin (s : State adder_hierarchical_4) (i : Fin 15) (hi : i.val = 0 := by decide) : evalExpr s (unrollDAG adder_hierarchical_4 15 i) = s ⟨0, by decide⟩ := by cases i; subst hi; rfl
+@[simp] lemma ast_adder_hierarchical_4_a_0 (s : State adder_hierarchical_4) (i : Fin 15) (hi : i.val = 1 := by decide) : evalExpr s (unrollDAG adder_hierarchical_4 15 i) = s ⟨1, by decide⟩ := by cases i; subst hi; rfl
+@[simp] lemma ast_adder_hierarchical_4_b_0 (s : State adder_hierarchical_4) (i : Fin 15) (hi : i.val = 2 := by decide) : evalExpr s (unrollDAG adder_hierarchical_4 15 i) = s ⟨2, by decide⟩ := by cases i; subst hi; rfl
+@[simp] lemma ast_adder_hierarchical_4_a_1 (s : State adder_hierarchical_4) (i : Fin 15) (hi : i.val = 3 := by decide) : evalExpr s (unrollDAG adder_hierarchical_4 15 i) = s ⟨3, by decide⟩ := by cases i; subst hi; rfl
+@[simp] lemma ast_adder_hierarchical_4_b_1 (s : State adder_hierarchical_4) (i : Fin 15) (hi : i.val = 4 := by decide) : evalExpr s (unrollDAG adder_hierarchical_4 15 i) = s ⟨4, by decide⟩ := by cases i; subst hi; rfl
+@[simp] lemma ast_adder_hierarchical_4_a_2 (s : State adder_hierarchical_4) (i : Fin 15) (hi : i.val = 5 := by decide) : evalExpr s (unrollDAG adder_hierarchical_4 15 i) = s ⟨5, by decide⟩ := by cases i; subst hi; rfl
+@[simp] lemma ast_adder_hierarchical_4_b_2 (s : State adder_hierarchical_4) (i : Fin 15) (hi : i.val = 6 := by decide) : evalExpr s (unrollDAG adder_hierarchical_4 15 i) = s ⟨6, by decide⟩ := by cases i; subst hi; rfl
+@[simp] lemma ast_adder_hierarchical_4_a_3 (s : State adder_hierarchical_4) (i : Fin 15) (hi : i.val = 7 := by decide) : evalExpr s (unrollDAG adder_hierarchical_4 15 i) = s ⟨7, by decide⟩ := by cases i; subst hi; rfl
+@[simp] lemma ast_adder_hierarchical_4_b_3 (s : State adder_hierarchical_4) (i : Fin 15) (hi : i.val = 8 := by decide) : evalExpr s (unrollDAG adder_hierarchical_4 15 i) = s ⟨8, by decide⟩ := by cases i; subst hi; rfl
+@[simp] lemma ast_adder_hierarchical_4_sum_0 (s : State adder_hierarchical_4) (i : Fin 15) (hi : i.val = 9 := by decide) : evalExpr s (unrollDAG adder_hierarchical_4 15 i) = (compute_adder_2 (s ⟨0, by decide⟩) (s ⟨1, by decide⟩) (s ⟨3, by decide⟩) (s ⟨2, by decide⟩) (s ⟨4, by decide⟩)).testBit 0 := by cases i; subst hi; rfl
+@[simp] lemma ast_adder_hierarchical_4_sum_1 (s : State adder_hierarchical_4) (i : Fin 15) (hi : i.val = 10 := by decide) : evalExpr s (unrollDAG adder_hierarchical_4 15 i) = (compute_adder_2 (s ⟨0, by decide⟩) (s ⟨1, by decide⟩) (s ⟨3, by decide⟩) (s ⟨2, by decide⟩) (s ⟨4, by decide⟩)).testBit 1 := by cases i; subst hi; rfl
+@[simp] lemma ast_adder_hierarchical_4_sum_2 (s : State adder_hierarchical_4) (i : Fin 15) (hi : i.val = 12 := by decide) : evalExpr s (unrollDAG adder_hierarchical_4 15 i) = (compute_adder_2 ((compute_adder_2 (s ⟨0, by decide⟩) (s ⟨1, by decide⟩) (s ⟨3, by decide⟩) (s ⟨2, by decide⟩) (s ⟨4, by decide⟩)).testBit 2) (s ⟨5, by decide⟩) (s ⟨7, by decide⟩) (s ⟨6, by decide⟩) (s ⟨8, by decide⟩)).testBit 0 := by cases i; subst hi; rfl
+@[simp] lemma ast_adder_hierarchical_4_sum_3 (s : State adder_hierarchical_4) (i : Fin 15) (hi : i.val = 13 := by decide) : evalExpr s (unrollDAG adder_hierarchical_4 15 i) = (compute_adder_2 ((compute_adder_2 (s ⟨0, by decide⟩) (s ⟨1, by decide⟩) (s ⟨3, by decide⟩) (s ⟨2, by decide⟩) (s ⟨4, by decide⟩)).testBit 2) (s ⟨5, by decide⟩) (s ⟨7, by decide⟩) (s ⟨6, by decide⟩) (s ⟨8, by decide⟩)).testBit 1 := by cases i; subst hi; rfl
+@[simp] lemma ast_adder_hierarchical_4_cout (s : State adder_hierarchical_4) (i : Fin 15) (hi : i.val = 14 := by decide) : evalExpr s (unrollDAG adder_hierarchical_4 15 i) = (compute_adder_2 ((compute_adder_2 (s ⟨0, by decide⟩) (s ⟨1, by decide⟩) (s ⟨3, by decide⟩) (s ⟨2, by decide⟩) (s ⟨4, by decide⟩)).testBit 2) (s ⟨5, by decide⟩) (s ⟨7, by decide⟩) (s ⟨6, by decide⟩) (s ⟨8, by decide⟩)).testBit 2 := by cases i; subst hi; rfl
+
+instance instIsAdder_adder_hierarchical_4 : IsAdder adder_hierarchical_4 4 a_bus_adder_hierarchical_4 b_bus_adder_hierarchical_4 sum_bus_adder_hierarchical_4 cin_adder_hierarchical_4 cout_adder_hierarchical_4 where
+  widths_match := by decide
+  inputs_are_valid := by intro i h; fin_cases h <;> rfl
+  adder_correct := by
+    intro s
+    have equiv (i : Fin 15) : evalCombinatorial adder_hierarchical_4 adder_hierarchical_4.gates.length s i = evalExpr s (unrollDAG adder_hierarchical_4 15 i) := by fin_cases i <;> rfl
+    simp only [a_bus_adder_hierarchical_4, b_bus_adder_hierarchical_4, sum_bus_adder_hierarchical_4, cout_adder_hierarchical_4, cin_adder_hierarchical_4, bitsToNat]
+    simp only [equiv]
+    simp only [ast_adder_hierarchical_4_cin, ast_adder_hierarchical_4_a_0, ast_adder_hierarchical_4_b_0, ast_adder_hierarchical_4_a_1, ast_adder_hierarchical_4_b_1, ast_adder_hierarchical_4_a_2, ast_adder_hierarchical_4_b_2, ast_adder_hierarchical_4_a_3, ast_adder_hierarchical_4_b_3, ast_adder_hierarchical_4_sum_0, ast_adder_hierarchical_4_sum_1, ast_adder_hierarchical_4_sum_2, ast_adder_hierarchical_4_sum_3, ast_adder_hierarchical_4_cout]
+    generalize h_cin : s ⟨0, by decide⟩ = cin
+    generalize h_a_0 : s ⟨1, by decide⟩ = a_0
+    generalize h_b_0 : s ⟨2, by decide⟩ = b_0
+    generalize h_a_1 : s ⟨3, by decide⟩ = a_1
+    generalize h_b_1 : s ⟨4, by decide⟩ = b_1
+    generalize h_a_2 : s ⟨5, by decide⟩ = a_2
+    generalize h_b_2 : s ⟨6, by decide⟩ = b_2
+    generalize h_a_3 : s ⟨7, by decide⟩ = a_3
+    generalize h_b_3 : s ⟨8, by decide⟩ = b_3
+    cases cin <;> cases a_0 <;> cases b_0 <;> cases a_1 <;> cases b_1 <;> cases a_2 <;> cases b_2 <;> cases a_3 <;> cases b_3 <;> decide
+
+instance instVerifiedAdder4_adder_hierarchical_4 : VerifiedAdder4 adder_hierarchical_4 a_bus_adder_hierarchical_4 b_bus_adder_hierarchical_4 sum_bus_adder_hierarchical_4 cin_adder_hierarchical_4 cout_adder_hierarchical_4 where
+  proof := instIsAdder_adder_hierarchical_4
+
+-- COMPONENT: adder_cla_2
+def adder_cla_2_gates : List Gate := [
+  Gate.mk .igate false,
+  Gate.mk .igate false,
+  Gate.mk .igate false,
+  Gate.mk .igate false,
+  Gate.mk .igate false,
+  Gate.mk .xor_ false,
+  Gate.mk .and_ false,
+  Gate.mk .xor_ false,
+  Gate.mk .and_ false,
+  Gate.mk .and_ false,
+  Gate.mk .or_ false,
+  Gate.mk .and_ false,
+  Gate.mk .and_ false,
+  Gate.mk .and_ false,
+  Gate.mk .or_ false,
+  Gate.mk .or_ false,
+  Gate.mk .xor_ false,
+  Gate.mk .xor_ false
+]
+def adder_cla_2_conns : List (List Nat) := [
+  [],
+  [],
+  [],
+  [],
+  [],
+  [1, 2],
+  [1, 2],
+  [3, 4],
+  [3, 4],
+  [5, 0],
+  [6, 9],
+  [7, 6],
+  [7, 5],
+  [12, 0],
+  [8, 11],
+  [14, 13],
+  [5, 0],
+  [7, 10]
+]
+def adder_cla_2 : Circuit := { gates := adder_cla_2_gates, wiring := mkWiring adder_cla_2_gates adder_cla_2_conns (by decide), is_dag := by decide }
+def a_bus_adder_cla_2 : List (Fin 18) := [⟨1, by decide⟩, ⟨3, by decide⟩]
+def b_bus_adder_cla_2 : List (Fin 18) := [⟨2, by decide⟩, ⟨4, by decide⟩]
+def sum_bus_adder_cla_2 : List (Fin 18) := [⟨16, by decide⟩, ⟨17, by decide⟩]
+def cin_adder_cla_2 : Fin 18 := ⟨0, by decide⟩
+def cout_adder_cla_2 : Fin 18 := ⟨15, by decide⟩
+
+-- AST BOUNDARY LEMMAS & PROOF: adder_cla_2
+@[simp] lemma ast_adder_cla_2_cin (s : State adder_cla_2) (i : Fin 18) (hi : i.val = 0 := by decide) : evalExpr s (unrollDAG adder_cla_2 18 i) = s ⟨0, by decide⟩ := by cases i; subst hi; rfl
+@[simp] lemma ast_adder_cla_2_a_0 (s : State adder_cla_2) (i : Fin 18) (hi : i.val = 1 := by decide) : evalExpr s (unrollDAG adder_cla_2 18 i) = s ⟨1, by decide⟩ := by cases i; subst hi; rfl
+@[simp] lemma ast_adder_cla_2_b_0 (s : State adder_cla_2) (i : Fin 18) (hi : i.val = 2 := by decide) : evalExpr s (unrollDAG adder_cla_2 18 i) = s ⟨2, by decide⟩ := by cases i; subst hi; rfl
+@[simp] lemma ast_adder_cla_2_a_1 (s : State adder_cla_2) (i : Fin 18) (hi : i.val = 3 := by decide) : evalExpr s (unrollDAG adder_cla_2 18 i) = s ⟨3, by decide⟩ := by cases i; subst hi; rfl
+@[simp] lemma ast_adder_cla_2_b_1 (s : State adder_cla_2) (i : Fin 18) (hi : i.val = 4 := by decide) : evalExpr s (unrollDAG adder_cla_2 18 i) = s ⟨4, by decide⟩ := by cases i; subst hi; rfl
+@[simp] lemma ast_adder_cla_2_sum_0 (s : State adder_cla_2) (i : Fin 18) (hi : i.val = 16 := by decide) : evalExpr s (unrollDAG adder_cla_2 18 i) = ((s ⟨1, by decide⟩ ^^ s ⟨2, by decide⟩) ^^ s ⟨0, by decide⟩) := by cases i; subst hi; rfl
+@[simp] lemma ast_adder_cla_2_sum_1 (s : State adder_cla_2) (i : Fin 18) (hi : i.val = 17 := by decide) : evalExpr s (unrollDAG adder_cla_2 18 i) = ((s ⟨3, by decide⟩ ^^ s ⟨4, by decide⟩) ^^ ((s ⟨1, by decide⟩ && s ⟨2, by decide⟩) || ((s ⟨1, by decide⟩ ^^ s ⟨2, by decide⟩) && s ⟨0, by decide⟩))) := by cases i; subst hi; rfl
+@[simp] lemma ast_adder_cla_2_cout (s : State adder_cla_2) (i : Fin 18) (hi : i.val = 15 := by decide) : evalExpr s (unrollDAG adder_cla_2 18 i) = (((s ⟨3, by decide⟩ && s ⟨4, by decide⟩) || ((s ⟨3, by decide⟩ ^^ s ⟨4, by decide⟩) && (s ⟨1, by decide⟩ && s ⟨2, by decide⟩))) || (((s ⟨3, by decide⟩ ^^ s ⟨4, by decide⟩) && (s ⟨1, by decide⟩ ^^ s ⟨2, by decide⟩)) && s ⟨0, by decide⟩)) := by cases i; subst hi; rfl
+
+instance instIsAdder_adder_cla_2 : IsAdder adder_cla_2 2 a_bus_adder_cla_2 b_bus_adder_cla_2 sum_bus_adder_cla_2 cin_adder_cla_2 cout_adder_cla_2 where
+  widths_match := by decide
+  inputs_are_valid := by intro i h; fin_cases h <;> rfl
+  adder_correct := by
+    intro s
+    have equiv (i : Fin 18) : evalCombinatorial adder_cla_2 adder_cla_2.gates.length s i = evalExpr s (unrollDAG adder_cla_2 18 i) := by fin_cases i <;> rfl
+    simp only [a_bus_adder_cla_2, b_bus_adder_cla_2, sum_bus_adder_cla_2, cout_adder_cla_2, cin_adder_cla_2, bitsToNat]
+    simp only [equiv]
+    simp only [ast_adder_cla_2_cin, ast_adder_cla_2_a_0, ast_adder_cla_2_b_0, ast_adder_cla_2_a_1, ast_adder_cla_2_b_1, ast_adder_cla_2_sum_0, ast_adder_cla_2_sum_1, ast_adder_cla_2_cout]
+    generalize h_cin : s ⟨0, by decide⟩ = cin
+    generalize h_a_0 : s ⟨1, by decide⟩ = a_0
+    generalize h_b_0 : s ⟨2, by decide⟩ = b_0
+    generalize h_a_1 : s ⟨3, by decide⟩ = a_1
+    generalize h_b_1 : s ⟨4, by decide⟩ = b_1
+    cases cin <;> cases a_0 <;> cases b_0 <;> cases a_1 <;> cases b_1 <;> decide
+
+instance instVerifiedAdder2_adder_cla_2 : VerifiedAdder2 adder_cla_2 a_bus_adder_cla_2 b_bus_adder_cla_2 sum_bus_adder_cla_2 cin_adder_cla_2 cout_adder_cla_2 where
+  proof := instIsAdder_adder_cla_2
+
+end hdl.examples.adder
